prove PackedKV relationship between SizeOfV and BucketWeight

lib/Buckets/BucketWeights.i.dfy
@@ -97,6 +97,21 @@ module BucketWeights {
     )
   }
 
+  function WeightList(keys: seq<Key>, messages: seq<Message>) : (result: nat)
+  {
+    if |keys| == 0 then
+      0
+    else
+      WeightList(DropLast(keys), DropLast(messages)) + WeightKey(Last(keys)) + WeightMessage(Last(messages))
+  }
+
+  lemma WeightListEqualsWellFormedWeightBucket(bucket: Bucket)
+    requires WFBucket(bucket)
+    requires BucketWellMarshalled(bucket)
+    ensures WeightList(bucket.keys, bucket.msgs) == WeightBucket(bucket)
+  {
+  }
+  
   function {:opaque} WeightBucketList(buckets: BucketList) : (w:int)
   ensures w >= 0
   {
