lib/Buckets/PackedStringArray.i.dfy
@@ -861,7 +861,7 @@ module PackedStringArray {
     {
       4 + 4 * nstrings + if nstrings == 0 then 0 else offsets[nstrings-1] as uint64
     }
-    
+
     predicate canAppend(str: Key)
       requires WF()
       reads this, this.Repr
